VsaIris.lean
@@ -41,3 +41,4 @@ import VsaIris.Vsa.Exit
 import VsaIris.Vsa.SegImg
 import VsaIris.Vsa.StdioRead
 import VsaIris.Vsa.MainErr
+import VsaIris.Vsa.Landing
